\documentclass{article}
\usepackage{graphicx} 
\usepackage{enumitem} 
\usepackage{amsmath}
\usepackage{amsmath, amssymb}

\setlength{\parindent}{0pt}

\title{RA Math Test: Exercise 1 \& Exercise 2}
\author{YILONG LIU}
\date{May 2025}

\begin{document}

\maketitle

\section{Exercise 1, Question 1: An unbiased estimator of the variance of i.i.d random variables}
Let $(Y_i)_{1\leq i \leq n}$ be n i.i.d random variables. Let $\bar{Y} = \frac{1}{n} \sum^n_{i=1}{Y_i}$ denote the average of these variables. Let $Y$ be a random variable with the same distribution as the $Y_i$s. The goal of the exercise is to show that $\frac{1}{n-1} \sum^n_{i=1}{(Y_i - \bar{Y})^2}$ is an unbiased estimator of $V(Y)$, the variance of the $Y_i$s.
\begin{enumerate}[label=(\arabic*), leftmargin=*, align=left]
    \item Show that 
    $\frac{1}{n-1} \sum^n_{i=1} (Y_i - \bar{Y})^2 = \frac{1}{n-1}\sum^n_{i=1}{Y^2_i}-\frac{n}{n-1}(\bar{Y})^2$.

    \item Use the result in question 1) to prove that 
    $E\left(\frac{1}{n-1} \sum^n_{i=1}(Y_i-\bar{Y})^2\right)=V(Y)$.
\end{enumerate}

\subsection{Question (1) Solution}
We can expand the left hand side equation and have:
\begin{align*}
\frac{1}{n-1} \sum^n_{i=1} (Y_i-\bar{Y})^2 &= \frac{1}{n-1}\sum^n_{i=1}(Y^2_i-2 Y_i \bar{Y}+\bar{Y}^2)
\\&=\frac{1}{n-1} (\sum^n_{i=1} Y^2_i) - \frac{2}{n-1}\bar{Y}(\sum^n_{i=1} Y_i)+\frac{n}{n-1}\bar{Y}^2
\\&=\frac{1}{n-1}\sum^n_{i=1}Y^2_i - \frac{2}{n-1}\bar{Y}{n \bar{Y}} + \frac{n}{n-1}\bar{Y}^2
\\&=\frac{1}{n-1} \sum^n_{i=1}Y^2_i - \frac{n}{n-1}\bar{Y}^2
\end{align*}

\subsection{Quesiton (2) Solution}
According to the result in question (1), we have the following:
\begin{align*}
E[\frac{1}{n-1}\sum^n_{i=1}(Y_i - \bar{Y})^2] &= E[\frac{1}{n-1} \sum^n_{i=1}Y^2_i - \frac{n}{n-1}(\bar{Y})^2]
\\&=\frac{1}{n-1}E[\sum^n_{i=1}Y^2_i] - \frac{n}{n-1}E[\bar{Y}^2]
\\&=E[\frac{1}{n-1}\sum^n_{i=1}Y^2_i]-E[\frac{n}{n-1}\bar{Y}^2]
\\&=E[Y^2] - E^2[Y]
\end{align*}
\textit{Note: As $\frac{1}{n-1} \sum^n_{i=1}Y^2_i$ is the unbiased estimator of $E[Y^2]$.}

\section{Exercise 1, Question 2: A super consistent estimator}

Assume you observe an iid sample of $n$ random variables $(Y_i)_{1 \leq i \leq n}$ following the uniform distribution on $[0, \theta]$, where $\theta$ is an unknown strictly positive real number we would like to estimate. Let $Y$ be a random variable with the same distribution as the $Y_i$s.

\begin{enumerate}[label=(\arabic*), leftmargin=*, align=left]
    \item Compute $E(Y)$. Write $\theta$ as a function of $E(Y)$.
    \item Use question a) to propose an estimator $\hat{\theta}_{MM}$ for $\theta$ using the method of moments (reminder: that method amounts to replacing expectations by sample means).
    \item Show that $\hat{\theta}_{MM}$ is an asymptotically normal estimator of $\theta$, and show that its asymptotic variance is $4V(Y)$.
\end{enumerate}

\noindent Consider the following alternative estimator for $\theta$: $\hat{\theta}_{ML} = \max\limits_{1 \leq i \leq n} \{ Y_i \}$.

\begin{enumerate}[label=(\arabic*), start=4, leftmargin=*, align=left]
    \item Why does using $\hat{\theta}_{ML}$ to estimate $\theta$ sounds like a natural idea?
    \item Show that
    \[
    P(\hat{\theta}_{ML} \leq x) = \left\{
    \begin{array}{ll}
    0 & \text{if } x < 0 \\
    \left( \frac{x}{\theta} \right)^n & \text{if } x \in [0, \theta] \\
    1 & \text{if } x > \theta
    \end{array}
    \right.
    \]
    \item Use the result in question (5) to show that $n\left(\frac{\theta - \hat{\theta}_{ML}}{\theta}\right) \xrightarrow{d} U$, where $U$ follows an exponential distribution with parameter 1. \textit{Hint:} to prove this, you need to use the definition of convergence in distribution in your lecture notes. Also, use the fact that the cdf of an exponential distribution with parameter 1 is
\[
F(x) = \left\{
\begin{array}{ll}
0 & \text{if } x < 0 \\
1 - \exp(-x) & \text{if } x \geq 0
\end{array}
\right.
\]

    \item Which estimator is the best: $\hat{\theta}_{MM}$, or $\hat{\theta}_{ML}$?
    \item Illustrate this through a Monte-Carlo study. Draw 1000 iid realizations of variables following a uniform distribution on $[0,1]$ in Stata (you need to use the ``uniform()'' command), compute $\hat{\theta}_{MM}$ and $\hat{\theta}_{ML}$. What is the value of $\theta$ in this example? Which estimator is the closest to $\theta$?
    \item For any $q \in (0,1)$, let $t_q$ denote the $q^{th}$ quantile of the $\text{exp}(1)$ distribution: $t_q = F^{-1}(q)$. Show that 
    \[
    IC(\alpha) = \left[ \hat{\theta}_{ML}, \hat{\theta}_{ML} + \hat{\theta}_{ML} \frac{t_{1 - \alpha}}{n} \right]
    \]
    is a confidence interval for $\theta$ with asymptotic coverage $1 - \alpha$. You should use the result from the previous question and the Slutsky lemma. You can use without proving it the fact that $\hat{\theta}_{ML} \xrightarrow{P} \theta$ (actually, that directly follows from the fact $\hat{\theta}_{ML}$ is an $n$-consistent estimator of $\theta$).
\end{enumerate}

\subsection{Question (1) Solution}
By definition:
$$E[Y] = \int^{\theta}_{0}y\cdot f(y)dy$$
As it is uniform distribution: $f(y) = \frac{1}{\theta}$
Then we have the follows:
\begin{align*}
E[Y] &= \int^{\theta}_{0}\frac{y}{\theta}dy
\\&= \frac{1}{2\theta}\cdot y^2|^{\theta}_0
\\&=\frac{\theta}{2}
\end{align*}
Therefore, $E[Y] = \frac{\theta}{2}$, $\theta = 2E[Y]$.

\subsection{Question (2) Solution}
From (1), $\theta = 2E[Y]$, we propose that the estimator $\hat{\theta}_{MM}$ for $\theta$ to be:
$$\hat{\theta}_{MM} = \frac{2}{n} \sum^{n}_{i=1}Y_i$$
based on n random variables $(Y_i)_{1\leq i \leq n}$.

\subsection{Question (3) Solution}
From (1), $\theta = 2E[Y]$, we propose that the estimator $\hat{\theta}_{MM}$ for $\theta$ to be:
\[
\hat{\theta}_{MM} = \frac{2}{n} \sum^{n}_{i=1}Y_i
\]
based on $n$ random variables $(Y_i)_{1\leq i \leq n}$.

By the Central Limit Theorem, we have:
\[
\sqrt{n}\left(\frac{1}{n}\sum^{n}_{i=1}Y_i - E[Y]\right) \xrightarrow{d} \mathcal{N}(0, V(Y))
\]
which implies that
\[
\sqrt{n}(\hat{\theta}_{MM} - \theta) = \sqrt{n} \left( 2\bar{Y} - 2E[Y] \right) = 2\sqrt{n}(\bar{Y} - E[Y]) \xrightarrow{d} \mathcal{N}(0, 4V(Y)).
\]

Therefore, $\hat{\theta}_{MM}$ is an asymptotically normal estimator of $\theta$, and its asymptotic variance is $4V(Y)$.

\subsection{Question (4) Solution}
It is because that the random variables $(Y_i)_{1\leq i \leq n}$ follows a uniform distribution on $[0, \theta]$.
Therefore for any $i$ such that $1 \leq i \leq n$, we have $Y_i \in [0, \theta]$, and it is then a natural idea to assume the key parameter $\hat{\theta}_{ML} = max_{1\leq i \leq n} {Y_i}$.

\subsection{Question (5) Solution}
By definition, $P(\hat{\theta}_{ML} \leq x) = P(max_{1\leq i \leq n} \{Y_i\} \leq x)$, then:

if $x < 0$, then the probility is 0 as $Y_i \in [0, \theta] $ for any $i$.

if $x \in [0, \theta]$, then:
\begin{align*}
P(max_{1\leq i \leq n} \{Y_i\} \leq x) &= \Pi^{n}_{i=1} P(Y_i\leq x)
\\&= \Pi^n_{i=1} F(X)
\\&= (\frac{x-0}{\theta - 0})^n
\\&= (\frac{x}{\theta})^n
\end{align*}

if $x > \theta$, then the probability is 1 as $Y_i \in [0, \theta] $ for any $i$.
\subsection{Question (6) Solution}
According to the description, we have the following:
\[
n\left(\frac{\theta - \hat{\theta}_{ML}}{\theta}\right) = n\left(1 - \frac{\hat{\theta}_{ML}}{\theta}\right)
\]

Then, we have:
\begin{align*}
F\left(n\left(1 - \frac{\hat{\theta}}{\theta}\right) < x\right) 
&= F\left(\frac{\hat{\theta}}{\theta} > 1 - \frac{x}{n}\right) \\
&= 1 - F\left(\frac{\hat{\theta}}{\theta} < 1 - \frac{x}{n}\right) \\
&= 1 - \left(1 - \frac{x}{n}\right)^n
\end{align*}

Therefore,
\begin{align*}
\lim_{n \to \infty} F(x) 
&= \lim_{n \to \infty} \left[1 - \left(1 - \frac{x}{n} \right)^n \right] \\
&= 1 - \lim_{n \to \infty} \left(1 - \frac{x}{n} \right)^n \\
&= 1 - \lim_{n \to \infty} \exp \left[n \ln\left(1 - \frac{x}{n} \right)\right] \\
&= 1 - \lim_{h \to 0} \exp \left[ \frac{-x \ln(1 + h)}{h} \right] \\
&= 1 - \exp(-x)
\end{align*}

\textit{Note: $h = \frac{-x}{n}$}

\subsection{Question (7) and (8) Solution}
To evaluate which estimator is better, we consider their performance across 1000 simulations:

\begin{center}
\begin{tabular}{lccc}
\hline
Estimator & Mean Estimate & Standard Deviation & Min -- Max \\
\hline
$\hat{\theta}_{MM}$ & 1.000846 & 0.0177101 & 0.9523674 -- 1.052426 \\
$\hat{\theta}_{ML}$ & 0.998992 & 0.0009990 & 0.9935493 -- 0.9999998 \\
\hline
\end{tabular}
\end{center}

Although both estimators are consistent, their statistical properties differ:

- The method of moments estimator $\hat{\theta}_{MM}$ is unbiased and its average estimate is closer to the true value $\theta = 1$.

- The maximum likelihood estimator $\hat{\theta}_{ML}$ is biased (slightly underestimates $\theta$ on average), but it has a much smaller variance.

Therefore, in terms of bias, $\hat{\theta}_{MM}$ performs better. In terms of efficiency (i.e., lower variance), $\hat{\theta}_{ML}$ is superior. 

The choice of the "best" estimator depends on the criterion:

- If minimizing mean squared error (bias$^2$ + variance), $\hat{\theta}_{ML}$ is preferred because its variance is much smaller.

- If unbiasedness is prioritized, then $\hat{\theta}_{MM}$ is preferred.

Overall, for large $n$, the bias of $\hat{\theta}_{ML}$ becomes negligible, and its lower variance makes it the better estimator in most practical contexts.

\vspace{1em}

We draw a sample of size $n = 1000$ from the uniform distribution on $[0,1]$ using Stata's `uniform()` command.

The true value of the parameter is:
\[
\theta = 1.
\]

From the Stata output of one simulation:
\[
\hat{\theta}_{MM} = 0.98998555, \quad \hat{\theta}_{ML} = 0.99975073.
\]

In this sample, $\hat{\theta}_{ML}$ is closer to the true value $\theta = 1$ than $\hat{\theta}_{MM}$. This aligns with the simulation results in (6), which show that although $\hat{\theta}_{MM}$ is on average closer to $\theta$, its individual estimates fluctuate more due to higher variance. $\hat{\theta}_{ML}$, while slightly biased, tends to provide estimates with much lower dispersion.

\subsection{Question (9) Solution}
For any $q \in (0,1)$, let $t_q$ denote the $q^{th}$ quantile of the $\text{exp}(1)$ distribution, i.e. $t_q = F^{-1}(q)$. From question (6), we have shown that
\[
n\left(\frac{\theta - \hat{\theta}_{ML}}{\theta}\right) \xrightarrow{d} \text{Exp}(1),
\]
which implies that
\[
P\left(n\left(\frac{\theta - \hat{\theta}_{ML}}{\theta}\right) \leq t_{1-\alpha}\right) \to 1 - \alpha.
\]

This is equivalent to:
\[
P\left(\theta \leq \hat{\theta}_{ML} + \hat{\theta}_{ML} \cdot \frac{t_{1-\alpha}}{n}\right) \to 1 - \alpha.
\]

Hence, the asymptotic $(1 - \alpha)$ confidence interval for $\theta$ is given by:
\[
IC(\alpha) = \left[\hat{\theta}_{ML}, \ \hat{\theta}_{ML} + \hat{\theta}_{ML} \cdot \frac{t_{1 - \alpha}}{n} \right].
\]

This result follows by applying the convergence in distribution from (7) and the Slutsky lemma. Note that $\hat{\theta}_{ML} \xrightarrow{p} \theta$ since $\hat{\theta}_{ML}$ is an $n$-consistent estimator.

\section{Exercise 1, Question 3}
Assume you observe two sequences of random variables $(U_n)_{n \in \mathbb{N}}$ and $(V_n)_{n \in \mathbb{N}}$. Assume that $U_n \xrightarrow{P} l$ and $V_n \xrightarrow{P} l'$, where $l$ and $l'$ are two real numbers.

\begin{enumerate}
    \item Use the \textit{continuous mapping theorem} to prove that $U_n \times V_n \xrightarrow{P} l \times l'$.

    \item Use the \textit{Slutsky lemma} to prove that $U_n \times V_n \xrightarrow{P} l \times l'$. You need to use the two following facts:
    
    \begin{enumerate}
        \item[1.] If $X_n \xrightarrow{P} X$, then $X_n \xrightarrow{d} X$ (convergence in probability implies convergence in distribution)

        \item[2.] If $X_n \xrightarrow{d} x$ and $x$ is a real number, then $X_n \xrightarrow{P} x$ (convergence in distribution \textbf{towards a real number} implies convergence in probability towards that real number)
    \end{enumerate}
\end{enumerate}
\subsection{Question (1) Solution}
    To prove that $U_n \times V_n \xrightarrow{P} l \times l'$ using the \textit{continuous mapping theorem}, define the continuous function $g(x, y) = xy$ on $\mathbb{R}^2$. Since $U_n \xrightarrow{P} l$ and $V_n \xrightarrow{P} l'$, we have:
    \[
    (U_n, V_n) \xrightarrow{P} (l, l').
    \]
    Then, by the continuous mapping theorem:
    \[
    g(U_n, V_n) = U_n \cdot V_n \xrightarrow{P} g(l, l') = l \cdot l'.
    \]

\subsection{Question (2) Solution}
    To prove the same result using the \textit{Slutsky lemma}, we proceed in steps:
    \begin{itemize}
        \item Since $U_n \xrightarrow{P} l$ and $V_n \xrightarrow{P} l'$, from Fact 1, we know that:
        \[
        U_n \xrightarrow{d} l, \quad V_n \xrightarrow{d} l'.
        \]
        \item Then, using the known result that if $X_n \xrightarrow{d} x$ and $Y_n \xrightarrow{d} y$ with $x, y \in \mathbb{R}$, then $X_n Y_n \xrightarrow{d} xy$, we get:
        \[
        U_n V_n \xrightarrow{d} l l'.
        \]
        \item Now, since $l l'$ is a real number, we apply Fact 2:
        \[
        U_n V_n \xrightarrow{P} l l'.
        \]
    \end{itemize}

\newpage
Asymptotic variance of the estimator of the variance of iid random variables.
Let $(Y_i)_{1\leq i \leq n}$ be an iid sample of $n$ random variables with a 4th moment and with a strictly positive variance. Let $Y$ denote a random variable with the same distribution as the $Y_i$s. Let $\bar{Y} = \frac{1}{n} \sum^{n}_{i=1}Y_i$, and let $\bar{Y}^2 = \frac{1}{n} \sum^n_{i=1}Y^2_{i}$. Let $\hat{V}(Y) = \bar{Y}^2-(\bar{Y})^2$ be an estimator of $V(Y)$.

\section{Exercise 2 Question 1}Show that
\[
\sqrt{n} \left( 
\begin{pmatrix}
\overline{Y^2} \\
\overline{Y}
\end{pmatrix}
-
\begin{pmatrix}
E(Y^2) \\
E(Y)
\end{pmatrix}
\right)
\xrightarrow{d} \mathcal{N}(0, V_0),
\]
where
\[
V_0 = 
\begin{pmatrix}
V(Y^2) & \operatorname{cov}(Y^2, Y) \\
\operatorname{cov}(Y^2, Y) & V(Y)
\end{pmatrix}.
\]

\subsection{Question 1 Solution}
This result follows directly from the multivariate Central Limit Theorem (CLT), which states that for a vector of sample means of i.i.d.\ variables with finite second moments, the scaled difference between the sample means and their expectations converges in distribution to a multivariate normal distribution.

Let $X_i = (Y_i^2, Y_i)'$ be a 2-dimensional random vector. Then by the multivariate CLT,
\[
\sqrt{n} \left( 
\begin{pmatrix}
\overline{Y^2} \\
\overline{Y}
\end{pmatrix}
-
\begin{pmatrix}
E(Y^2) \\
E(Y)
\end{pmatrix}
\right)
\xrightarrow{d} \mathcal{N}(0, V_0),
\]
where $V_0$ is the covariance matrix of $X_i$.

\section{Exercise 2, Question 2} Use the previous question and a well-known theorem to prove that
\[
\sqrt{n} \left( \widehat{V}(Y) - V(Y) \right) \xrightarrow{d} \mathcal{N}(0, V_1),
\]
where
\[
V_1 = (1, -2E(Y)) V_0 (1, -2E(Y))'.
\]

\subsection{Question 2 Solution}
We know that the sample variance is defined as:
\[
\widehat{V}(Y) = \overline{Y^2} - \overline{Y}^2
\quad \text{and} \quad
V(Y) = E(Y^2) - (E(Y))^2
\]

Define the function $g(a, b) = a - b^2$. This is a differentiable function from $\mathbb{R}^2 \to \mathbb{R}$. By the delta method, since
\[
\sqrt{n} 
\begin{pmatrix}
\overline{Y^2} - E(Y^2) \\
\overline{Y} - E(Y)
\end{pmatrix}
\xrightarrow{d} \mathcal{N}(0, V_0),
\]
we apply the delta method with gradient $\nabla g(a, b) = (1, -2b)$. Evaluated at $(a, b) = (E(Y^2), E(Y))$, this becomes $(1, -2E(Y))$.

Hence,
\[
\sqrt{n} \left( \widehat{V}(Y) - V(Y) \right) \xrightarrow{d} \mathcal{N}\left(0, (1, -2E(Y)) V_0 (1, -2E(Y))' \right),
\]
which proves the result.

\section{Exercise 2, Question 3} In this question, we focus on the special case where the $Y_i$s are binary random variables. To alleviate the notation, let $p = E(Y)$. We have $V(Y) = p(1 - p)$. Moreover, in this special case $\widehat{V}(Y) = \overline{Y}(1 - \overline{Y})$.

\begin{enumerate}
    \item[(a)] Use the results from questions 1 and 2 to prove that $V_1 = p(1 - p)(1 - 2p)^2$.

    \item[(b)] For $p = \frac{1}{2}$, $p(1 - p) = \frac{1}{4}$, and $p(1 - p)(1 - 2p)^2 = 0$. Therefore, if $p = \frac{1}{2}$, what is the asymptotic distribution of $\sqrt{n} \left( \overline{Y}(1 - \overline{Y}) - \frac{1}{4} \right)$?

    \item[(c)] Show that $n\left( \overline{Y}(1 - \overline{Y}) - \frac{1}{4} \right) = \left( \sqrt{n} \left( \overline{Y} - \frac{1}{2} \right) \right)^2$, and use this equality to derive the asymptotic distribution of $n\left( \overline{Y}(1 - \overline{Y}) - \frac{1}{4} \right)$.

    \item[(d)] The previous questions show that the asymptotic distribution of $\sqrt{n} \left( \widehat{V}(Y) - V(Y) \right)$ depends on the value of $p$, which is unknown. Then, how could you build a confidence interval for $V(Y)$?
\end{enumerate}

\subsection{Question (a) Solution}
From question 2, we know that the asymptotic variance is given by:
\[
V_1 = (1, -2E(Y)) V_0 (1, -2E(Y))'
\]

In the binary case, $Y_i \in \{0, 1\}$:
\[
E(Y) = p, \quad E(Y^2) = E(Y) = p, \quad \Rightarrow V(Y) = p(1 - p)
\]
\[
V(Y^2) = p(1 - p), \quad \operatorname{cov}(Y^2, Y) = \operatorname{cov}(Y, Y) = V(Y) = p(1 - p)
\]

So the matrix $V_0$ becomes:
\[
V_0 = 
\begin{pmatrix}
p(1 - p) & p(1 - p) \\
p(1 - p) & p(1 - p)
\end{pmatrix}
\]

Now compute:
\[
V_1 = 
\begin{pmatrix}
1 & -2p
\end{pmatrix}
\begin{pmatrix}
p(1 - p) & p(1 - p) \\
p(1 - p) & p(1 - p)
\end{pmatrix}
\begin{pmatrix}
1 \\
-2p
\end{pmatrix}
\]

Performing the matrix multiplication:
\[
(1, -2p)
\begin{pmatrix}
p(1 - p)(1 - 2p) + (-2p)p(1 - p)
\end{pmatrix}
= p(1 - p)(1 - 2p)^2
\]

\subsection{Question (b) Solution}
When $p = \frac{1}{2}$:
\[
p(1 - p) = \frac{1}{4}, \quad (1 - 2p)^2 = 0
\]

From part (a), $V_1 = p(1 - p)(1 - 2p)^2 = 0$, so the asymptotic variance is zero. Therefore:
\[
\sqrt{n} \left( \overline{Y}(1 - \overline{Y}) - \frac{1}{4} \right) \xrightarrow{P} 0
\]

That is, the difference converges to zero faster than $1/\sqrt{n}$ â€” the asymptotic distribution is degenerate at 0.

\subsection{Question (c) Solution}
We expand:
\[
\overline{Y}(1 - \overline{Y}) = \overline{Y} - \overline{Y}^2 = \frac{1}{4} + \left( \overline{Y} - \frac{1}{2} \right) - \left( \overline{Y} - \frac{1}{2} \right)^2
\]

This simplifies to:
\[
\overline{Y}(1 - \overline{Y}) - \frac{1}{4} = -\left( \overline{Y} - \frac{1}{2} \right)^2
\Rightarrow
n \left( \overline{Y}(1 - \overline{Y}) - \frac{1}{4} \right) = -n \left( \overline{Y} - \frac{1}{2} \right)^2 = - \left( \sqrt{n} \left( \overline{Y} - \frac{1}{2} \right) \right)^2
\]

From the Central Limit Theorem:
\[
\sqrt{n} \left( \overline{Y} - \frac{1}{2} \right) \xrightarrow{d} \mathcal{N}(0, \tfrac{1}{4})
\Rightarrow
\left( \sqrt{n} \left( \overline{Y} - \frac{1}{2} \right) \right)^2 \xrightarrow{d} \frac{1}{4} \chi^2_1
\]

Thus:
\[
n \left( \overline{Y}(1 - \overline{Y}) - \frac{1}{4} \right) \xrightarrow{d} -\frac{1}{4} \chi^2_1
\]

\subsection{Question (d) Solution}
The asymptotic distribution of $\sqrt{n} (\widehat{V}(Y) - V(Y))$ depends on $p$, which is unknown. Since
\[
V_1 = p(1 - p)(1 - 2p)^2 = V(Y)(1 - 2p)^2,
\]
we can estimate $p$ by $\overline{Y}$ and substitute it into the asymptotic variance expression.

Therefore, an approximate $(1 - \alpha)$ confidence interval for $V(Y)$ is:
\[
\left[ \widehat{V}(Y) \pm z_{1 - \alpha/2} \cdot \frac{\sqrt{\widehat{V}(Y)}|1 - 2\overline{Y}|}{\sqrt{n}} \right]
\]
where $z_{1 - \alpha/2}$ is the standard normal quantile.
\end{document}
